theory/JITPer_mul_other.thy
@@ -42,8 +42,13 @@ lemma mulq_one_step_match_mem:
     storev M64 m1 (Vptr sp_block (xrs (IR SP) - (2::64 word) * u64_of_memory_chunk M64)) (Vlong (xrs (IR RDX))) = Some m2 \<Longrightarrow>
     loadv M64 m2 (Vptr sp_block (xrs (IR SP) - (2::64 word) * u64_of_memory_chunk M64)) = Some (Vlong (xrs (IR RDX))) \<Longrightarrow>
     loadv M64 m2 (Vptr sp_block (xrs (IR SP) - u64_of_memory_chunk M64)) = Some (Vlong (xrs (IR RAX))) \<Longrightarrow> match_mem m' m2"
-  apply (simp add: match_state_def match_mem_def eval_alu_def eval_reg_def)
-  using sp_block_def store_load_other_blk by auto
+  apply (simp add: match_state_def)
+  apply(subgoal_tac "m = m'")
+  prefer 2 
+  subgoal
+    apply(cases "eval_alu BPF_MUL dst (SOReg src) rs",simp_all)
+    done
+  using sp_block_def match_mem_def match_mem_store_1_equiv by blast
   
 lemma mulq_one_step_match_stack:
   " (SBPF_OK pc' rs' m') = sbpf_step prog (SBPF_OK pc rs m) \<Longrightarrow>
